SDP.lean
@@ -1,6 +1,7 @@
 -- This module serves as the root of the `SDP` library.
 -- Import modules here that should be built as part of the library.
 import SDP.Policy
+import SDP.Policy.Argmax
 import SDP.SDP
 import SDP.Trajectory
 import SDP.Value
