SDP/Policy/Argmax.lean
@@ -1,0 +1,45 @@
+
+import SDP.Value
+import SDP.SDP
+import SDP.Policy
+import SDP.Util.Argmax
+
+namespace Argmax
+
+open StateCtrl
+open PolicySeq
+
+variable {V : Type}
+variable [Value V]
+variable {m : Type → Type}
+variable [Monad m]
+variable [sdp : SDP V m]
+
+variable (argmax : {t : Nat} → (s : State t) → Argmax (Ctrl s) V)
+
+/-- If `Argmax (Ctrl s) V` for every `s : State t` then one can define
+a policy extension function. -/
+
+def extFun : ExtFun :=
+  fun ps s =>
+    Argmax.argmax (self := (argmax s)) (val' ps s)
+
+/-- The policy extension function given by `extFun` is optimal. -/
+
+lemma IsOptExtFun_extFun : IsOptExtFun (extFun argmax) := by
+  repeat intro
+  rw [val_eq_val', val_eq_val' (p := extFun argmax _)]
+  apply Argmax.le_argmax
+
+/-- If `Argmax (Ctrl s) V` for every `s : State t` then one can construct a
+policy sequence of any length. -/
+
+def bestPolicySeq (t n : Nat) : PolicySeq t n :=
+  policySeq_from_ExtFun (extFun argmax) t n
+
+/-- The policy sequence `bestPolicySeq` is optimal. -/
+
+theorem optimal_bestPolicySeq : IsOptimalPolicySeq (bestPolicySeq argmax t n) := by
+  simp [bestPolicySeq]
+  apply OptPolicySeq_from_OptExtFun
+  apply IsOptExtFun_extFun
